
%%%%%%%%%%%%%%%%%%%%%%%%%%%%%%%%%%%%%%%%%%%%%%%%%%%%%%%%%%
%%
%% This is the "PREAMBLE". Here we define the type of document and load in any packages we might want. You can also set parameters %% % and create your own short-hand here.
%%
%%%%%%%%%%%%%%%%%%%%%%%%%%%%%%%%%%%%%%%%%%%%%%%%%%%%%%%%%%

\documentclass[9pt]{article}

\def\solutions{1}


\usepackage{amsmath}
\usepackage{amssymb}
\usepackage{graphicx}    % needed for including graphics e.g. EPS, PS \usepackage{tikz}
\usepackage{tikz}
\usepackage{tikzsymbols}
\usepackage{relsize}
\usetikzlibrary{patterns,decorations.pathreplacing,shapes,arrows}
\usepackage{algorithm2e}
\topmargin -2.5cm        % read Lamport p.163
\oddsidemargin -0.04cm   % read Lamport p.163
\evensidemargin -0.04cm  % same as oddsidemargin but for left-hand pages
\textwidth 16.59cm
\textheight 25.94cm
% \pagestyle{empty}        % Uncomment if don't want page numbers
\pagenumbering{gobble}
\parskip 7.2pt           % sets spacing between paragraphs
%\renewcommand{\baselinestretch}{1.5} 	% Uncomment for 1.5 spacing between lines
\parindent 0pt		  % sets leading space for paragraphs

% No date in header
\date{}

\usepackage{hyperref}
\hypersetup{
colorlinks=true,
linkcolor=blue,
filecolor=magenta,      
urlcolor=cyan,
}
\usepackage{amsthm}
\usepackage{fancyhdr}
\usepackage{hyperref}
\usepackage{listings}
\lstset{escapeinside={||},
mathescape=true}



\pagestyle{fancy}
\setlength{\headsep}{36pt}



\newcommand{\lp}{\left(}
\newcommand{\rp}{\right)}
\newcommand{\lb}{\left[}
\newcommand{\rb}{\right]}
\newcommand{\ls}{\left\{}
\newcommand{\rs}{\right\}}
\newcommand{\lbar}{\left|}
\newcommand{\rbar}{\right|}
\newcommand{\ld}{\left.}
\newcommand{\rd}{\right.}

\newcommand{\myexists}{\exists \hspace{.3mm}}

\newcommand{\hs}{\hspace{.75mm}}
\newcommand{\bs}{\hspace{-.75mm}}
\newcommand{\nin}{\noindent}

\newcommand{\fx}{f\bs\left( x \right)}
\newcommand{\gx}{g\bs\left( x \right)}
\newcommand{\qx}{q\bs\left( x \right)}

\newcommand{\nn}{\nonumber}

\newcommand{\vfive}{\vspace{5mm}}
\newcommand{\vthree}{\vspace{3mm}}

\newcommand{\fof}[1]{f\lp #1\rp}
\newcommand{\gof}[1]{g\lp #1\rp}
\newcommand{\qof}[1]{q\lp #1\rp}

\newcommand{\myp}[1]{\left( #1 \right)}
\newcommand{\myb}[1]{\left[ #1 \right]}
\newcommand{\mys}[1]{\left\{ #1 \right\}}
\newcommand{\myab}[1]{\left| #1 \right|}

\newcommand{\myj}{_j}
\newcommand{\myjp}{_{j+1}}
\newcommand{\myjm}{_{j-1}}

\newcommand{\f}[1]{f\hspace{-1mm}\left( #1 \right)}
\newcommand{\fp}[1]{f'\hspace{-1mm}\left( #1 \right)}
\newcommand{\g}[1]{g\hspace{-1mm}\left( #1 \right)}
\newcommand{\gp}[1]{g'\hspace{-1mm}\left( #1 \right)}
\newcommand{\q}[1]{q\hspace{-1mm}\left( #1 \right)}
\newcommand{\qp}[1]{q'\hspace{-1mm}\left( #1 \right)}
\newcommand{\Px}[1]{P\hspace{-1mm}\left( x_{#1} \right)}
\newcommand{\Qx}[1]{Q\hspace{-1mm}\left( x_{#1} \right)}

\newcommand{\tten}[1]{\times 10^{#1}}

\newcommand{\aij}[1]{a_{#1}}
\newcommand{\bij}[1]{b_{#1}}
\newcommand{\rij}[1]{r_{#1}}

\newcommand{\R}[1]{\mathbb{R}^{#1}}

\newcommand{\ith}{i^{\textrm{th}}}
\newcommand{\jth}{i^{\textrm{th}}}
\newcommand{\kth}{i^{\textrm{th}}}

\newcommand{\inv}[1]{{#1}^{-1}}

\newcommand{\bx}{\mathbf{x}}
\newcommand{\bv}{\mathbf{v}}
\newcommand{\bw}{\mathbf{w}}
\newcommand{\by}{\mathbf{y}}
\newcommand{\bb}{\mathbf{b}}
\newcommand{\be}{\mathbf{e}}
\newcommand{\br}{\mathbf{r}}
\newcommand{\xhat}{\hat{\mathbf{x}}}

\newcommand{\beq}{\begin{eqnarray}}
    \newcommand{\eeq}{\end{eqnarray}}
    
    \newcommand{\ben}{\begin{enumerate}}
        \newcommand{\een}{\end{enumerate}}
        
        \newcommand{\bsq}{\mathsmaller{\blacksquare}}
        
        \newcommand{\iter}[1]{^{\myp{#1}}}
        
        % matrix macro
        \newcommand{\mymat}[1]{
        \left[
        \begin{array}{rrrrrrrrrrrrrrrrrrrrrrrrrrrrrrrrrrrrrrr}
            #1
        \end{array}
        \right]
        }
        
        \newcommand{\makenonemptybox}[2]{%
        %\par\nobreak\vspace{\ht\strutbox}\noindent
        \item[]
        \fbox{% added -2\fboxrule to specified width to avoid overfull hboxes
        % and removed the -2\fboxsep from height specification (image not updated)
        % because in MWE 2cm is should be height of contents excluding sep and frame
        \parbox[c][#1][t]{\dimexpr\linewidth-2\fboxsep-2\fboxrule}{
        \hrule width \hsize height 0pt
        #2
        }%
        }%
        \par\vspace{\ht\strutbox}
        }
        \makeatother
        
        \newcommand{\smallaug}[1]{
        \left[
        \begin{array}{rr|r}
            #1
        \end{array}
        \right]
        }
        
        %%%%%%%%%%%%%%%%%%%%%%%%%%%%%%%%%%%%%%%%%%%%%%%%%%%%%%%%%%
        %%
        %% End of PREAMBLE
        %%
        %%%%%%%%%%%%%%%%%%%%%%%%%%%%%%%%%%%%%%%%%%%%%%%%%%%%%%%%%%
        
        
        
        % ======================================================================================
        % Actual document starts here. 
        % PLEASE FILL IN YOUR NAME AND STUDENT ID.
        % ======================================================================================
        \begin{document}
        
        \lhead{{\bf CSCI 3104, Algorithms \\ Problem Set 1 (50 points)} }
        \rhead{Name: \fbox{Jaryd Meek}  \\  ID: \fbox{} \\ Collaborators: Noah Nguyen \\ {\bf Due January 22, 2021 \\ Spring 2021, CU-Boulder}}
        \renewcommand{\headrulewidth}{0.5pt}
        
        \phantom{Test}
        
        \begin{small}
            \textit{Advice 1}:\ For every problem in this class, you must justify your answer:\ show how you arrived at it and why it is correct. If there are assumptions you need to make along the way, state those clearly.
            \vspace{-3mm} 
            
            \textit{Advice 2}:\ Verbal reasoning is typically insufficient for full credit. Instead, write a logical argument, in the style of a mathematical proof.\\
            \vspace{-3mm} 
            
            \textbf{Instructions for submitting your solution}:
            \vspace{-5mm} 
            
            \begin{itemize}
                \item The solutions \textbf{should be typed} and we cannot accept hand-written solutions. \href{http://ece.uprm.edu/~caceros/latex/introduction.pdf}{Here's a short intro to Latex.}
                \item You should submit your work through \href{https://www.gradescope.com/courses/218966}{\textbf{Gradescope}} only.
                \item The easiest way to access Gradescope is through our Canvas page. There is a Gradescope button in the left menu.
                \item Gradescope will only accept \textbf{.pdf} files.
                \item \href{https://www.youtube.com/watch?v=u-pK4GzpId0&feature=emb_logo}{It is vital that you match each problem part with your work.} Skip to 1:40 to just see the matching info.
            \end{itemize}
            \vspace{-4mm} 
        \end{small}
        
        \hrulefill
        \pagebreak
        
        
        
        \ben
        %%%%%%%%%%%%%%%%%%%%%%%%%%%%%%%%%%%%%%%%%%%%%%%%%%%%%%%%
        % PROBLEM  ONE %% PROBLEM  ONE %% PROBLEM  ONE %% PROBLEM  ONE %% PROBLEM  ONE %
        %==============================================================================
        % Problem 1: Loop invariants and Induction Review
        %==============================================================================
        % PROBLEM  ONE %% PROBLEM  ONE %% PROBLEM  ONE %% PROBLEM  ONE %% PROBLEM  ONE %
        %%%%%%%%%%%%%%%%%%%%%%%%%%%%%%%%%%%%%%%%%%%%%%%%%%%%%%%%
        
        \item
        
        \begin{enumerate}
            
            \item Identify and describe the components of a loop invariant proof.
            \item Identify and describe the components of a mathematical induction proof.
        \end{enumerate}
        
        \if\solutions1
        \vspace{2mm}
        
        \textbf{Solution:}   \\
        %==============================================================================
        % STUDENTS: TYPE YOUR SOLUTIONS HERE. (Between \textbf{Solution:} and \fi )
        %==============================================================================
        
        \begin{enumerate}
            \item 
            \begin{enumerate}
                \item \textbf{Initialization -} 
                Describes what is true prior to the first iteration of the loop.
                \item \textbf{Maintenance -} 
                Describes how if the loop invariant is true before the iteration of the loop, it is also true after an iteration of the loop.
                \item \textbf{Termination -} 
                When the loop hits it's termination point, the invariant gives us information to prove that the algorithm is correct.
            \end{enumerate}
            \bigskip\bigskip
            \item 
            \begin{enumerate}
                \item \textbf{Base Case -} 
                In the base case you verify that the given statement or equation holds for the first item in the set.
                \item \textbf{Induction Step -} 
                In the induction step, you prove that since it worked for the $n$ case, it also works for the $n+1$ case.
                \item \textbf{Conclusion -} 
                State that since the induction step proved true, the statement is true for all $n$.
            \end{enumerate}
        \end{enumerate}
        
        \fi
        
        \newpage
        
        
        %%%%%%%%%%%%%%%%%%%%%%%%%%%%%%%%%%%%%%%%%%%%%%%%%%%%%%%%
        % PROBLEM TWO %% PROBLEM TWO %% PROBLEM TWO %% PROBLEM TWO %% PROBLEM TWO %
        %==============================================================================
        % Problem 2: Identify Loop Invariant
        %==============================================================================
        % PROBLEM TWO %% PROBLEM TWO %% PROBLEM TWO %% PROBLEM TWO %% PROBLEM TWO %
        %%%%%%%%%%%%%%%%%%%%%%%%%%%%%%%%%%%%%%%%%%%%%%%%%%%%%%%%
        
        
        
\vspace{5mm}
\item
Identify the loop invariant for the following algorithms.

\begin{enumerate}
\item 
\begin{small}
\begin{lstlisting}
|\textbf{function}| Sum(|\textbf{A}|)
    answer=0;
    n=length(|\textbf{A}|);
    |\textbf{for}| i=1 to n
        answer += |\textbf{A}|[i]
    |\textbf{end}|
    |\textbf{return}| answer
|\textbf{end}|
\end{lstlisting}	
\end{small}





\item 
\begin{small}
\begin{lstlisting}
|\textbf{function}| Reverse(|\textbf{A}|)
    n=length(|\textbf{A}|)
    i=ceiling(n/2)
    j=ceiling(n/2) + (n+1) mod 2
    |\textbf{while}| i>0 and j<=n
        tmp=|\textbf{A}|[i]
        |\textbf{A}|[i]=|\textbf{A}|[j]
        |\textbf{A}|[j]=tmp
        i=i-1
        j=j+1
    |\textbf{end}|
|\textbf{end}|
\end{lstlisting}	
\end{small}

\item 
Assume that \textbf{A}  is sorted such that the largest value is at \textbf{A}[n].  Assume \textbf{A} contains the value \verb target .
\begin{small}
\begin{lstlisting}
|\textbf{function}| Search(|\textbf{A}|,target) //returns the index of the value target
    left=1
    right=length(|\textbf{A}|)
    |\textbf{while}| left <=right
        m=floor((left+right)/2)
        |\textbf{if} \textbf{A}|[m] < target
            left=m+1
        |\textbf{else if A}|[m]>target
            right=m-1
        |\textbf{else}|
            |\textbf{return}| m
        |\textbf{end}|
    |\textbf{end}|
|\textbf{end}|
\end{lstlisting}
\end{small}

\end{enumerate}



\if\solutions1
\vspace{2mm}

\textbf{Solution:} \\
        %==============================================================================
        % STUDENTS: TYPE YOUR SOLUTIONS HERE. (Between \textbf{Solution:} and \fi )
        %==============================================================================
        \begin{enumerate}
            \item At the start of iteration $i$, the variable \verb answer  will have the sum of the values in the subarry $A[1 : (i-1)]$.
            
            \item At the start of each iteration, the subarray $A[i+1 : j-1]$ will contain the items from the original array, in reverse order.
            
            \item At the start of each iteration, the subarray $A[left : right]$ will contain the \verb target .
        \end{enumerate}
        
        \fi
        \newpage
        
        
        %%%%%%%%%%%%%%%%%%%%%%%%%%%%%%%%%%%%%%%%%%%%%%%%%%%%%%%%
        % PROBLEM THREE %% PROBLEM THREE %% PROBLEM THREE %% PROBLEM THREE %% PROBLEM THREE %
        %==============================================================================
        % Problem 3: Loop Invariant Proof
        %==============================================================================
        % PROBLEM THREE %% PROBLEM THREE %% PROBLEM THREE %% PROBLEM THREE %% PROBLEM THREE %
        %%%%%%%%%%%%%%%%%%%%%%%%%%%%%%%%%%%%%%%%%%%%%%%%%%%%%%%%
        
        \vspace{5mm}
        
        \item 
        Prove the correctness of the following algorithm. (\textit{Hint: You need to prove the correctness of the inner loop before you can prove the correctness of the outer loop.})
        
\begin{small}
\begin{lstlisting}
|\textbf{function}| Sort(|\textbf{A}|)
    n=length(|\textbf{A}|) 
    |\textbf{for}| i=1 to n
        |\textbf{for}| j=2 to n
            |\textbf{if}| |\textbf{A}|[j]<|\textbf{A}|[j-1]
                swap(|\textbf{A}|[j],|\textbf{A}|[j-1]) //a function that swaps the elements in the array
            |\textbf{end}|
        |\textbf{end}|
    |\textbf{end}|
|\textbf{end}|
\end{lstlisting}
\end{small}
        
        \if\solutions1
        \vspace{2mm}
        
        \textbf{Solution:} \\
        %==============================================================================
        % STUDENTS: TYPE YOUR SOLUTIONS HERE. (Between \textbf{Solution:} and \fi )
        %==============================================================================
        
        \textbf{Inner Loop -}\\
        \textit{Loop Invariant - } Prior to iteration $j$, the value of $A[j-1]$ is the largest in the subarray $A[1 : j-1]$\\
        
        \textit{Initialization - } The loop initializes at $j=2$. This tells us that $A[2-1] = A[1]$ is the largest value in the subarray $A[1:2-1] = A[1:1]$. Since $A[1:1]$ is just a single value, with that value being $A[1]$, $A[1]$ must be the largest value.\\
        
        \textit{Maintenence - } At the start of the $j^{\text{th}}$ iteration, the subarray $A[1 : j-1]$ has the largest value at $A[j-1]$. We examine $A[j]$ to determine if it is less than $A[j-1]$. If it is, we swap the two. This maintains that the largest value will be at the position of $A[j-1]$, thus the loop invariant is maintained. \\
        
        \textit{Termination - } At the start of the last loop $j=n$, we assume that the loop invariant holds before the last iteration and that $A[n-1]$ is the largest value in the subarray $A[1 : n-1]$. After using the maintenance step, we get that $A[j-1] = A[n]$ is the largest value in the array $A[1 : n]$ and we terminate. \\
        
        \textbf{Outer Loop -}\\
        \textit{Loop Invariant - } Prior to iteration $i$, the subarray $A[n-(i-1) : n]$ is sorted. \\
        
        \textit{Initialization - } The loop initializes at $i=1$. This tells us that $A[n-(i-1) : n] = A[n-(1-1) : n] = A[n : n]$ which is an array of one item and is therefore sorted. \\
        
        \textit{Maintenence - } At the start of the $i^{\text{th}}$ iteration, $A[n-(i-1) : n]$ is sorted. Thus when iteration i+1 starts, the inner for loop moves the greatest value in the subarray $A[1 : n-i]$ to the rightmost position. This means that the subarray $A[n-i : n]$ will be sorted. Therefore the loop invariant is maintained. \\
        
        \textit{Termination - } At the start of the last loop, $i=n$. We assume that the loop invariant holds before the last iteration, meaning that $A[2 : n]$ is sorted.  Using the maintainence step, we get that $A[1: n]$ is sorted. $i$ then incriments and we terminate with $A$ sorted.\\
        \fi
        
        \newpage
        
        
        
        
        %==============================================================================
        % Problem 4: Induction Proofs
        %==============================================================================
        \vspace{5mm}
        
        \item
        
        
        
        \begin{enumerate}
            
            \item Suppose you have a whole chocolate bar composed of $n\geq 1$ individual pieces.  Prove that the minimum number of breaks to divide the chocolate bar into $n$ pieces is $n-1$. 
            
            \item{
            Show that for fibonacci numbers $\sum_{i=1}^n f_i^2 = f_{n}f_{n+1}$\\
            Recall that the fibonacci numbers are defined as \\
            $f_0 = 0,\ f_1=1$ \\
            $\forall n>1$, $f_n=f_{n-1} + f_{n-2}$}
            
            \item For which nonnegative integers $n$ is $3n+2 \leq 2^n$? Prove your answer.
            
        \end{enumerate}
        
        \if\solutions1
        \vspace{3mm}
        
        {\bf Solution}: \\
        %==============================================================================
        % STUDENTS: TYPE YOUR SOLUTIONS HERE. (Between \textbf{Solution:} and \fi )
        %==================================================================
        
        \begin{enumerate}
            \item \textbf{Proof by weak induction -} \\
            \textit{Base Case -} \\ 
            If there is 1 piece of chocolate, there are 0 breaks since there is only a single square of chocolate. (like you just got it out of the wrapper)\\
            
            $$\text{number of breaks} = n-1 = 1-1 = 0$$
            $$0 \stackrel{\text{\checkmark}}{=} 0 $$\\

            \textit{Inductive Step -} \\
            \textit{Inductive Hypothesis -}
            Assume that every chocolate bar with $n$ pieces has $n-1$ breaks. \\
            Let $C$ be a chocolate bar with $n+1$ pieces.\\
            Let $C'$ be a chocolate bar with one less piece.\\
            $C'$ has $n$ pieces, By the inductive hypothesis, $C'$ has $n-1$ breaks.\\
            Thus, $C$ has $n+1$ pieces and $n$ breaks because it has one more break than $C'$
            \\

            \textit{Conclusion -} \\
            Since $n$ was arbitrary, we've shown that all chocolate bars with with $n$ pieces have $n-1$ breaks
            
            \item \textbf{Proof by weak induction -} \\
            \textit{Base Case -}\\ $$n = 2$$ 
            $$\sum_{i=1}^{2} f_i^2 = f_1^2 + f_2^2 = 1^2  + 1^2 = 2$$
            $$f_{2} \cdot f_{3} = 1 \cdot 2 = 2$$
            $$2 \stackrel{\text{\checkmark}}{=} 2 $$ 

            \textit{Inductive Step -} \\
            Assume that $\sum_{i=1}^{n} f_i^2 = f_{i} \cdot f_{i+1}$ for some $n \geq 2$\\
            \begin{equation*}
                \begin{split}
                    \sum_{i=1}^{n+1} f_i^2 & = \sum_{i=1}^{n} f_i^2 + f_{n+1}^2\text{~~~~\quad \quad (By properties of sums)}\\
                    & = f_n \cdot f_{n+1} + f_{n+1}^2\text{~\quad \quad (By inductive hypothesis)}\\
                    & = f_{n+1} \left(f_n+ f_{n+1}\right)\text{\quad \quad (Factor out a }f_{n+1}\text{)}\\
                    & = f_{n+1} \cdot f_{n+2} \text{\quad\quad\quad~~\quad (Simplify }f_n + f_{n+1}\text{ to } f_{n+2} \text{ using definiton of fibonacci numbers)}
                \end{split} 
            \end{equation*}

            \textit{Conclusion -} \\Therefore by weak induction, we've shown that $\forall n>1, \sum_{i=1}^n f_i^2 = f_{n} \cdot f_{n+1} $
            \newpage

            \item \textbf{Proof by weak induction -} \\
            \textit{Base Case -} \\
            $$n=4$$
            $$(3 \cdot 4) + 2 = 14$$
            $$2^4 = 16$$
            $$14 \stackrel{\text{\checkmark}}{\leq} 16 $$ 

            \textit{Inductive Step -} \\
            Assume that $3k+2 \leq 2^k$ for all $k \geq 4$
            $$\textbf{Substitute k+1 in and simplify}$$
            $$3(k+1) + 2 \leq 2^{k+1}$$
            $$3k+5 \leq 2^{k+1}$$
            
            $$\textbf{Solve the original equation for k+1}$$
            $$3k + 2 \leq 2^{k}\text{\quad \quad (start with the inductive hypothesis)}$$
            $$2(3k+2)\leq 2^{k}\cdot 2\text{\quad \quad (multiply both sides by 2)}$$
            $$6k+4\leq 2^{k+1}\text{\quad \quad (distribute the left, simplify the right)}$$
            $$\text{Ok, since we have that } 6k+4\leq 2^{k+1}\text{ Ok, since we have that }$$
            $$6k+4\leq 2^{k+1}\text{\quad \quad (distribute the left, simplify the right)}$$

            $$\textbf{Properties of inequalities}$$
            $$\text{since } 3k+5 \leq 2^{k+1}$$
            $$\text{and } 6k+4 \leq 2^{k+1}$$
            $$\text{and } 3k+5 \leq 6k+5 \quad \forall k \geq 4$$
            $$\therefore 3k+5 \leq 6k+4 \leq 2^{k+1}$$
            \\
            \textit{Conclusion -}
            Since we have shown above that when you substitute $k+1$ into the original equation, you get that $2^{k+1}$ must be greater than $3k+5$ and below we've shown that $2^{k+1}$ must also be greater than $6k+4$, and $6k+4$ must always be greater than $3k+5$ (since we're working with all numbers greater than 4), we've shown that $\forall n \geq 4, 3n+2 \leq 2^n$ 
        \end{enumerate}
        
        \fi
        
        
        %========================================================================================================================
        
        \een 
        
        
        \end{document}
        